@prefix bibo:    <http://purl.org/ontology/bibo/> .
@prefix dcterms: <http://purl.org/dc/terms/> .
@prefix foaf:    <http://xmlns.com/foaf/0.1/> .
@prefix odrl:    <http://www.w3.org/ns/odrl/2/> .
@prefix owl:     <http://www.w3.org/2002/07/owl#> .
@prefix rdf:     <http://www.w3.org/1999/02/22-rdf-syntax-ns#> .
@prefix rdfs:    <http://www.w3.org/2000/01/rdf-schema#> .
@prefix report:  <https://w3id.org/force/compliance-report#> .
@prefix skos:    <http://www.w3.org/2004/02/skos/core#> .
@prefix sotw:    <https://w3id.org/force/sotw#> .
@prefix vann:    <http://purl.org/vocab/vann/> .
@prefix xsd:     <http://www.w3.org/2001/XMLSchema#> .

# ---------------- Ontology Metadata ------------------ #

<https://w3id.org/force/sotw> a owl:Ontology ;
    dcterms:title "Contextual Inputs for ODRL Evaluators"@en ;
    vann:preferredNamespacePrefix "sotw" ;
    vann:preferredNamespaceUri "https://w3id.org/force/sotw#" ;
    rdfs:label "Contextual Inputs for ODRL Evaluators"@en ;
    owl:versionInfo "0.2" ;
    owl:versionIRI <https://w3id.org/force/sotw/0.2> ;
    dcterms:created "2025-08-12"^^xsd:date ;
    dcterms:modified "2025-12-18"^^xsd:date ;
    dcterms:issued "2025-12-18"^^xsd:date ;
    dcterms:creator <https://solidweb.me/besteves4/profile/card#me>,
        <https://pod.woutslabbinck.com/profile/card#me>,
        <#andrea> ;
    dcterms:publisher <https://data.knows.idlab.ugent.be/person/office/#> ;
    dcterms:abstract "Vocabulary used to represent state of the world and evaluation requests, which are necessary inputs for ODRL evaluators."@en ;
    dcterms:description "Vocabulary used to represent state of the world and evaluation requests, which are necessary inputs for ODRL evaluators."@en ;
    rdfs:comment "This is the Turtle serialisation for the Contextual Inputs for ODRL Evaluators specification."@en ;
    dcterms:bibliographicCitation "Cite this vocabulary as: Esteves, B., Slabbinck, W. (2025). Contextual Inputs for ODRL Evaluators specification (Version 0.1). https://doi.org/XXX"@en ;
    bibo:doi "xxxxx"@en ;
    # foaf:logo <https://github.com/SolidLabResearch/ODRL-Compliance-Report-Model/blob/main/img/Compliance%20Report%20Model.svg> ;
    dcterms:source <http://www.w3.org/ns/odrl/2/>, <https://w3c.github.io/odrl/formal-semantics/> ;
    dcterms:license <https://creativecommons.org/licenses/by-sa/4.0/> .

### State of the World concepts ###

sotw:SotW a rdfs:Class, owl:Class, skos:Concept ;
    rdfs:isDefinedBy sotw: ;
    rdfs:label "State of the World"@en ;
    skos:definition "Knowledge representing real-world information aiding the evaluation of ODRL Policies"@en .

sotw:context a rdfs:Property, skos:Concept ;
    rdfs:label "Context"@en ;
    rdfs:isDefinedBy sotw: ;
    skos:definition "Denotes contextual information related to the state of the world"@en ;
    rdfs:domain sotw:SotW ;
    rdfs:range rdfs:Resource .

sotw:conditionID a rdfs:Property, skos:Concept ;
    rdfs:isDefinedBy sotw: ;
    rdfs:label "Condition ID"@en ;
    skos:definition "Denotes a relationship between a certain SotW context and a particular rule, constraint or duty"@en ;
    skos:example "Link contextual information about a payment to a duty to pay within a permission to use a certain asset"@en ;
    rdfs:domain rdfs:Resource ;
    rdfs:range odrl:Rule, odrl:Constraint .

### Evaluation Request concepts ###

sotw:EvaluationRequest a rdfs:Class, owl:Class, skos:Concept ;
    rdfs:isDefinedBy sotw: ;
    rdfs:label "Evaluation Request"@en ;
    skos:definition "An Evaluation Request represents a formal description of a requested action by an assignee on a target asset, which can be enriched with further contextual information"@en .

sotw:RequestParameter a rdfs:Class, owl:Class, skos:Concept ;
    rdfs:isDefinedBy sotw: ;
    rdfs:label "Request Parameter"@en ;
    skos:definition "An Request Parameter represents additional contextual information that can be included in the Evaluation Request"@en ;
    skos:example "A request to translate an asset to a certain language or to use an asset for a certain purpose"@en .

sotw:DataFeature a rdfs:Class, owl:Class, skos:Concept ;
    rdfs:isDefinedBy sotw: ;
    rdfs:label "Data Feature"@en ;
    skos:definition "A Data Feature describes a certain parameter that is being assessed in the Request Parameter"@en ;
    skos:example "Temporal data can be a data feature. As such, the request parameter should expect a date type value related to this feature"@en .

sotw:evaluatedAction a rdfs:Property, skos:Concept ;
    rdfs:isDefinedBy sotw: ;
    rdfs:label "Evaluated Action"@en ;
    skos:definition "Denotes the requested action to be evaluated"@en ;
    rdfs:domain sotw:EvaluationRequest ;
    rdfs:range odrl:Action .

sotw:evaluatedParty a rdfs:Property, skos:Concept ;
    rdfs:isDefinedBy sotw: ;
    rdfs:label "Evaluated Party"@en ;
    skos:definition "Denotes the party being evaluated in relation to the evaluated action"@en ;
    rdfs:domain sotw:EvaluationRequest ;
    rdfs:range odrl:Party .

sotw:evaluatedTarget a rdfs:Property, skos:Concept ;
    rdfs:isDefinedBy sotw: ;
    rdfs:label "Evaluated Target"@en ;
    skos:definition "Denotes the asset being evaluated in relation to the evaluated action"@en ;
    rdfs:domain sotw:EvaluationRequest ;
    rdfs:range odrl:Asset .

sotw:requestParameter a rdfs:Property, skos:Concept ;
    rdfs:isDefinedBy sotw: ;
    rdfs:label "Request Parameter"@en ;
    skos:definition "Denotes additional contextual information that MAY be included in the request to be evaluated"@en ;
    rdfs:domain sotw:EvaluationRequest ;
    rdfs:range sotw:RequestParameter .

sotw:describesFeature a rdfs:Property, skos:Concept ;
    rdfs:isDefinedBy sotw: ;
    rdfs:label "Describes Feature"@en ;
    skos:definition "Describes the data feature that is being assessed in the request parameter"@en ;
    rdfs:domain sotw:RequestParameter ;
    rdfs:range sotw:DataFeature .

sotw:value a rdfs:Property, skos:Concept ;
    rdfs:label "Value"@en ;
    rdfs:isDefinedBy sotw: ;
    skos:definition "Attributes a value to the data feature"@en ;
    rdfs:domain sotw:RequestParameter .