@prefix bibo:          <http://purl.org/ontology/bibo/> .
@prefix dcterms:       <http://purl.org/dc/terms/> .
@prefix foaf:          <http://xmlns.com/foaf/0.1/> .
@prefix odrl:          <http://www.w3.org/ns/odrl/2/> .
@prefix odrl3proposal: <https://w3id.org/force/odrl3proposal#> .
@prefix owl:           <http://www.w3.org/2002/07/owl#> .
@prefix rdf:           <http://www.w3.org/1999/02/22-rdf-syntax-ns#> .
@prefix rdfs:          <http://www.w3.org/2000/01/rdf-schema#> .
@prefix sh:             <http://www.w3.org/ns/shacl#>.
@prefix skos:          <http://www.w3.org/2004/02/skos/core#> .
@prefix vann:          <http://purl.org/vocab/vann/> .
@prefix xsd:           <http://www.w3.org/2001/XMLSchema#> .

# ---------------- Ontology Metadata ------------------ #

<https://w3id.org/force/odrl3proposal> a owl:Ontology ;
    dcterms:title "Open Digital Rights Language (ODRL) 3.0 Proposal"@en ;
    vann:preferredNamespacePrefix "odrl3proposal" ;
    vann:preferredNamespaceUri "https://w3id.org/force/odrl3proposal#" ;
    rdfs:label "Open Digital Rights Language (ODRL) 3.0 Proposal"@en ;
    owl:versionInfo "0.1" ;
    # owl:versionIRI <https://w3id.org/force/odrl3proposal/0.1> ;
    dcterms:created "2025-05-13"^^xsd:date ;
    # dcterms:modified "2025-xx-xx"^^xsd:date ;
    dcterms:issued "2025-05-13"^^xsd:date ;
    dcterms:creator <https://solidweb.me/besteves4/profile/card#me>,
        <https://pod.woutslabbinck.com/profile/card#me>,
        <https://wouter.termont.online/>,
        <https://data.knows.idlab.ugent.be/person/joachimvh/#me> ;
    dcterms:publisher <https://data.knows.idlab.ugent.be/person/office/#> ;
    dcterms:abstract ""@en ;
    dcterms:description ""@en ;
    rdfs:comment "This is the Turtle serialisation for the ODRL 3.0 Proposal specification."@en ;
    dcterms:bibliographicCitation "Cite this vocabulary as: Esteves, B., Slabbinck, W., Termont, W., Van Herwegen, J. (2025). Open Digital Rights Language (ODRL) 3.0 Proposal (Version 0.1). https://doi.org/xxxx"@en ;
    bibo:doi "xxxxx"@en ;
    # foaf:logo <https://github.com/SolidLabResearch/ODRL-Compliance-Report-Model/blob/main/img/Compliance%20Report%20Model.svg> ;
    dcterms:source <http://www.w3.org/ns/odrl/2/>, <https://w3c.github.io/odrl/formal-semantics/> ;
    dcterms:license <https://creativecommons.org/licenses/by-sa/4.0/> .

# ---------------- Classes ------------------ #

odrl3proposal:OperandReference a rdfs:Class, skos:Concept ;
    rdfs:label "Operand Rerefence"@en ;
    rdfs:isDefinedBy odrl3proposal: ;
    skos:definition "The `Operand Reference` class is used to to represent a Right Operand Value that has to be dynamically be materialized based on its properties."@en .

# ---------------- Properties ------------------ #

odrl3proposal:relation a rdf:Property, skos:Concept ;
    rdfs:label "relation"@en ;
    rdfs:isDefinedBy odrl3proposal: ;
    skos:definition "The `relation` property is used to classify the relation between the `odrl:Asset`s that are `odrl:partOf` a `odrl:AssetCollection` and the `odrl:source` of said collection."@en ;
    rdfs:domain odrl:AssetCollection ; 
    rdfs:range rdf:Property .

odrl3proposal:scope a rdf:Property, skos:Concept ;
    rdfs:label "scope"@en ;
    rdfs:isDefinedBy odrl3proposal: ;
    skos:definition "The `scope` property indicates the actions on which a `odrl:Policy`, with the subject `odrl:Asset` as `odrl:target`, can be defined."@en ;
    rdfs:domain odrl:Asset ; 
    rdfs:range odrl:Action .

odrl3proposal:path a rdf:Property, skos:Concept ;
    rdfs:label "path"@en ;
    rdfs:isDefinedBy odrl3proposal: ;
    skos:definition "The `path` property indicates the SHACL Property Path which describes the path from a specific focus node to a value it describes."@en ;
    skos:scopeNote "ODRL Core Vocabulary Terms"@en ;
    rdfs:domain odrl3proposal:OperandReference ;
    rdfs:range sh:path .

odrl3proposal:reference a rdf:Property, skos:Concept ;
    rdfs:label "reference"@en ;
    rdfs:isDefinedBy odrl3proposal: ;
    skos:definition "The `reference` property indicates the SHACL Property Path which describes the path from a specific focus node to a value it describes."@en ;
    rdfs:domain odrl3proposal:OperandReference ;
    rdfs:range xsd:anyURI .